function_utils.v
@@ -3,6 +3,7 @@ Require Import eval LibHypsNaming Memory.
 Require Import Errors.
 Require Import Cminor.
 Require Import spark2Cminor.
+Require Import compcert_utils.
 
 
 Open Scope Z_scope.
